Major refactoring

ident.v
@@ -1,39 +1,12 @@
-Require Import ssreflect ssrnat ssrbool seq eqtype Ring.
+Require Import ssreflect ssrnat ssrbool seq eqtype Ring Group.
 
-Module Import RingFacts := Ring.RingMT.
-Context (ZZ : Type) .
-Context (group_mul : ZZ -> ZZ -> ZZ) (groupinv : ZZ -> ZZ) (Id : ZZ).
+Module SteinbergGroup <: GroupCarrier.
+Variable ZZ : Type.
+End SteinbergGroup.
 
-Notation "x ^-1" := (groupinv x) (at level 40).
-Notation "x .* y " := (group_mul x y) (at level 50, left associativity).
-
-Definition Comm (x y : ZZ) : ZZ := (x .* y .* x^-1 .* y^-1).
-Notation "[ ~ x1 , x2 , .. , xn ]" :=
-  (Comm .. (Comm x1 x2) .. xn) (at level 29, left associativity).
-
-Axiom GId: forall g, g .* Id = g.
-Axiom IdG: forall g, Id .* g = g.
-Axiom GA : forall g1 g2 g3, g1 .* g2 .* g3 = g1 .* (g2 .* g3).
-
-Axiom GI : forall g, g .* (g ^-1) = Id.
-Corollary GI' g A: g .* ((g ^-1) .* A) = A. by rewrite -GA GI IdG. Qed.
-Axiom IG: forall g, (g ^-1) .* g = Id.
-Corollary IG' g A: (g^-1) .* (g .* A) = A. by rewrite -GA IG IdG. Qed.
-
-Lemma GC: forall g3 g1 g2, g1 .* g3 = g2 .* g3 -> g1 = g2.
-intros. have: (g1 .* g3 .* g3 ^-1 = g2 .* g3 .* g3 ^-1) by rewrite H.
-by rewrite ?GA ?GI ?GId. Qed.
-
-Lemma GIM: forall g1 g2, (g1 .* g2) ^-1 = g2 ^-1 .* g1 ^-1.
-intros. apply (GC (g1 .* g2)). by rewrite IG GA -(GA (g1 ^-1)) IG IdG IG. Qed.
-
-Lemma GII: forall g, g ^-1 ^-1 = g.
-intros. apply (GC (g^-1)). by rewrite IG GI. Qed.
-
-Lemma IdI: Id ^-1 = Id. apply (GC Id). by rewrite IG IdG. Qed.
-
-Lemma Comm_inv: forall x y, [~ x, y] ^-1 = [~y, x].
-intros. by rewrite /Comm ?GIM ?GII -?GA. Qed.
+Module Import GF := Group.GroupFacts SteinbergGroup.
+Module Import RF := Ring.RingFacts.
+Import SteinbergGroup.
 
 (* ********************************************** *)
 
@@ -43,14 +16,6 @@ Definition swap_neq {i j : nat}: i != j -> j != i. by rewrite eq_sym.  Defined.
 Lemma swapI {i j : nat} (p : i != j): swap_neq (swap_neq p) = p. Admitted. 
 
 Axiom X: forall {i j : nat}, (i != j) -> R -> ZZ.
-Definition pow (h g : ZZ) := (g ^-1) .* h .* g.
-Notation "h ^ g" := (pow h g).
-
-Lemma pow_mul h g1 g2: h ^ (g1 .* g2) = (h ^ g1) ^ g2.
-by rewrite /pow ?GIM ?GA. Qed.
-Lemma mul_pow g h1 h2: (h1 .* h2) ^ g = h1 ^ g .* h2 ^ g.
-by rewrite /pow ?GA -(GA g) GI IdG. Qed.
-Lemma powId g: g ^ Id = g. by rewrite /pow IdI IdG GId. Qed.
 
 Definition Z {i j : nat} (p : i != j) (r s : R) := (X p r) ^ (X (swap_neq p) s).
 
@@ -75,17 +40,14 @@ Lemma ST1': forall {i j k : nat} (ij : (i != j)) (ik : (i != k)) (jk : (j != k))
  [~ X jk r , X ij s ] = X ik (- s * r).
 intros. by rewrite -Comm_inv ST1 -ST0' inv_mul. Qed.
 
-Lemma pow_com: forall a b, a ^ b = [~ b ^-1, a] .* a. 
-intros. rewrite /pow. apply (GC Id). by rewrite -{1}(IG a) -GA /Comm GII GId. Qed. 
-
 Lemma ST2': forall {i j k} (ik : i != k) (jk : j != k) (ij : i != j) a b, X ik a ^ X jk b = X ik a.
-intros. rewrite pow_com -ST0' ST2. by rewrite IdG. exact (swap_neq ik). exact jk. Qed.
+intros. rewrite conj_com -ST0' ST2. by rewrite IdG. exact (swap_neq ik). exact jk. Qed.
 
 Lemma ST2'': forall {i j k} (ki : k != i) (kj : k != j) (ij : i != j) a b, X ki a ^ X kj b = X ki a.
-intros. rewrite pow_com -ST0' ST2. by rewrite IdG. exact (swap_neq kj). exact ki. Qed.
+intros. rewrite conj_com -ST0' ST2. by rewrite IdG. exact (swap_neq kj). exact ki. Qed.
 
 Lemma Zinv {i j} (ij : i != j) (r s : R): Z ij (-r) s = (Z ij r s)^-1.
-by rewrite /Z /pow ST0' ?GIM ?GA GII. Qed.
+by rewrite /Z /conj ST0' ?GIM ?GA GII. Qed.
 
 Lemma R10 i j k a b c: forall (ij : i!=j) (ik : i!=k) (jk : j!=k),
 let RHS := 
@@ -95,30 +57,30 @@ let RHS :=
 .* (X (swap_neq jk) (c * a) .* X ij a) in
  Z ij a (b * c) = RHS.
 intros. rewrite /Z. set ji := swap_neq ij. set ki := swap_neq ik.  set kj := swap_neq jk.
-rewrite -(ST1 jk ji ki) /Comm ?pow_mul (pow_com (X ij a)) -ST0' ST1' mul_pow inv_mul mul_inv invI
-        (pow_com (X ij a)) -ST0' (ST1 ki kj ij) inv_mul.
-rewrite 2!(mul_pow (X jk (-b))) Zdef' -(pow_mul). replace (swap_neq jk) with kj by done.
+rewrite -(ST1 jk ji ki) /Comm ?conj_mul (conj_com (X ij a)) -ST0' ST1' mul_conj inv_mul mul_inv invI
+        (conj_com (X ij a)) -ST0' (ST1 ki kj ij) inv_mul.
+rewrite 2!(mul_conj (X jk (-b))) Zdef' -(conj_mul). replace (swap_neq jk) with kj by done.
 replace (X ki c .* X jk (-b)) with ([~ X ki c, X jk (-b)] .* X jk (-b) .* X ki c); 
  [|by rewrite /Comm ?GA -(GA (X jk (- b) ^-1)) IG IdG IG GId].
-rewrite (ST1' jk ji ki) invI ?pow_mul (pow_com (X ik (a * b))) -ST0' ST1 inv_mul.
-rewrite (mul_pow (X jk (- b))) {3}/pow -ST0' invI -2!ST0 (plus_comm b) plus_assoc inv_r plus_1_r. 
-rewrite ST2'; [|exact ij]. rewrite (mul_pow (X ki c)) Zdef (pow_com _ (X ki c)) -ST0' ST1' invI mul_inv.
-rewrite (pow_com (X ij a)) -ST0' invI ST1'.
+rewrite (ST1' jk ji ki) invI ?conj_mul (conj_com (X ik (a * b))) -ST0' ST1 inv_mul.
+rewrite (mul_conj (X jk (- b))) {3}/conj -ST0' invI -2!ST0 (plus_comm b) plus_assoc inv_r plus_1_r. 
+rewrite ST2'; [|exact ij]. rewrite (mul_conj (X ki c)) Zdef (conj_com _ (X ki c)) -ST0' ST1' invI mul_inv.
+rewrite (conj_com (X ij a)) -ST0' invI ST1'.
 remember (Z ik (a*b) c) as Z1. remember (Z kj (-(c*a)) (-b)) as Z2.
-rewrite -?GA ?mul_pow HeqZ1 HeqZ2 {HeqZ1 HeqZ2 Z1 Z2}.
-rewrite {1}/Z -pow_mul. replace (swap_neq ik) with ki; [|done]. rewrite -ST0 inv_r Xzero powId Zdef.
-rewrite ST2'; [|exact jk]. rewrite (pow_com _ (X ki (- c))) -ST0' invI ST1' invI ST0' -GA IG IdG.
-rewrite {1}/Z -pow_mul swapI. 
+rewrite -?GA ?mul_conj HeqZ1 HeqZ2 {HeqZ1 HeqZ2 Z1 Z2}.
+rewrite {1}/Z -conj_mul. replace (swap_neq ik) with ki; [|done]. rewrite -ST0 inv_r Xzero conjId Zdef.
+rewrite ST2'; [|exact jk]. rewrite (conj_com _ (X ki (- c))) -ST0' invI ST1' invI ST0' -GA IG IdG.
+rewrite {1}/Z -conj_mul swapI. 
 replace (X jk (- b) .* X ki (- c)) with ([~X jk (- b), X ki (- c)] .* X ki (- c) .* X jk (- b));
   [|by rewrite /Comm ?GA -(GA (X ki (- c) ^-1)) IG IdG IG GId].
-rewrite ST1 inv_mul mul_inv invI (GA (X ji (b * c))) pow_mul (pow_com (X kj (- (c * a)))) -ST0' ST1' invI mul_inv mul_pow.
+rewrite ST1 inv_mul mul_inv invI (GA (X ji (b * c))) conj_mul (conj_com (X kj (- (c * a)))) -ST0' ST1' invI mul_inv mul_conj.
 assert (A0: X ki (- c) .* X jk (- b) = [~ X ki (- c) , X jk (- b)] .* X jk (- b) .* X ki (- c)) by by
  rewrite /Comm ?GA -(GA (X jk (- b) ^-1)) IG IdG IG GId.
-rewrite {1}A0 {A0} ST1' inv_mul mul_inv invI (pow_com (X ij a)) -ST0' invI ST1
-        (GA (X ji (- b * c))) pow_mul ST2'; [|exact kj].
-rewrite 2!pow_mul ST2''; [|exact ji].
-rewrite Zdef' (pow_com (X ki (- (c * a * (b * c))))) -ST0' invI ST1 mul_inv
-        mul_pow ST2' /pow;[|exact jk].
+rewrite {1}A0 {A0} ST1' inv_mul mul_inv invI (conj_com (X ij a)) -ST0' invI ST1
+        (GA (X ji (- b * c))) conj_mul ST2'; [|exact kj].
+rewrite 2!conj_mul ST2''; [|exact ji].
+rewrite Zdef' (conj_com (X ki (- (c * a * (b * c))))) -ST0' invI ST1 mul_inv
+        mul_conj ST2' /conj;[|exact jk].
 by rewrite -ST0' invI -?ST0 plus_comm -plus_assoc inv_l plus_1_l. Qed.
 
 Corollary R1 i j k a b c: forall (ij : i!=j) (ik : i!=k) (jk : j!=k),
@@ -128,7 +90,7 @@ X jk (- (b * c * a * b)) .* X ik (a * b) .* (X ji (- (b * c * a * b * c))
     .* X ki (- (c * a * b * c)) .* Z kj (- (c * a)) (- b)) .* Z ik (- (a * b)) (- c) .* X kj (c * a) .* X ij a.
 intros. move: (R10 i j k a b c ij ik jk). by rewrite -GA -?mul_assoc inv_mul. Qed.
 
-Ltac expand := rewrite /Comm /pow ?GIM ?GII.
+Ltac expand := rewrite /Comm /conj ?GIM ?GII.
 Ltac cancel := rewrite ?GI' ?IG' ?GI ?IG.
 Ltac cancellate := expand; rewrite ?GA; cancel.
 
@@ -136,33 +98,12 @@ Corollary R1F i j k a b c: forall (ij : i!=j) (ik : i!=k) (jk : j!=k),
 let ji := swap_neq ij in let ki := swap_neq ik in let kj := swap_neq jk in
  Z ij a (b * c) .* X ij (- a) .* X kj (- (c * a)) .*  Z ik (a * b) (- c) .* Z kj (c * a) (- b) .* 
  X ki (c * a * b * c) .* X ji (b * c * a * b * c) .* X ik (- (a * b)) .* X jk (b * c * a * b) = Id.
-intros. rewrite (R1 i j k) /Z /pow /ji /ki /kj ?ST0' ?GII ?GA. by do 4 cancel. Qed.
-
-Lemma HallWitt x y z: 
- [~ y^-1, x, z] ^ (y^-1) .* 
- [~ z^-1, y, x] ^ (z^-1) .* 
- [~ x^-1, z, y] ^ (x^-1) = Id. by expand; rewrite ?GA; do 4 cancel. Qed.
-
-Corollary HallWitt2 x y z: [~ y, x^-1, z^-1]^ y .* [~z, y^-1, x^-1]^ (z) .* [~x, z^-1, y^-1] ^ x = Id.
-move: (HallWitt (x^-1) (y^-1) (z^-1)). by rewrite ?GII. Qed.
-
-Lemma CL1 x y z: [~z, x, y]^ z = [~x, z^-1, y^z]. by cancellate. Qed.
-Lemma CL2 x y z: [~ x .* y, z] = [~y, z] ^ (x^-1) .* [~x, z]. by cancellate. Qed.
-Lemma CL3 x y z: [~ x, y .* z] = [~x, y] .* [~x, z] ^ (y^-1). by cancellate. Qed.
-Lemma CL4 x y z: [~ x, y] ^ z = [~x ^ z, y ^ z]. by cancellate. Qed.
-Lemma CL5 x y: [~ x, y] = y ^ (x^-1) .* y^-1. by expand. Qed.
-Lemma CL6 x y: [~ x, y] = x .* (x^-1) ^ (y^-1). by cancellate. Qed.
-
-
-Corollary HallWitt3 x y z: 
- [~ x^-1, y^-1, (z^-1)^y] .* 
- [~ y^-1, z^-1, (x^-1)^z] .* 
- [~ z^-1, x^-1, (y^-1)^x] = Id. by rewrite -?CL1 HallWitt2. Qed.
+intros. rewrite (R1 i j k) /Z /conj /ji /ki /kj ?ST0' ?GII ?GA. by do 4 cancel. Qed.
 
 Definition HW x y z := [~x, y, z^(y^-1)] .*  [~y, z, x^(z^-1)] .*  [~z, x, y^(x^-1)].
 
 Corollary HallWitt4 x y z: HW x y z = Id.
-move: (HallWitt3 (x^-1) (y^-1) (z^-1)). by rewrite /HW ?GII. Qed.
+move: (HallWitt'' (x^-1) (y^-1) (z^-1)). by rewrite /HW ?GII. Qed.
 
 Lemma R10' i j k (a b c : R): forall (ij : i!=j) (ik : i!=k) (jk : j!=k),
 let ji := swap_neq ij in let ki := swap_neq ik in let kj := swap_neq jk in
@@ -174,12 +115,12 @@ Z ij a (- (b * c)) .* X ij (- a) .* X ki (- (c * a * b * c))
 .* X jk (- (b * c * a * b)) .* X ji (b * c * a * b * c) in Id = RHS.
 
 intros. assert (A0: HW (X jk b) (X ki c) (X ij a) = Id). apply HallWitt4.
-move: A0. rewrite /HW ?ST1 ?pow_com -?ST0' ?GII ?invI ?ST1 ?CL3 
- ST1' (ST1' ik) (ST1' ji) ?CL4 -?ST0' ?ST2' ?pow_com -?ST0' ?invI ?ST1 ?mul_inv ?inv_mul -?mul_assoc
- ?CL2 // (ST1 ki) (ST1 ij) (ST1 jk) /pow -?ST0' ?invI.
-remember ([ ~ X ji (b * c), X ij a]) as W1. rewrite CL5 -?ST0' Zdef in HeqW1.
-remember ([ ~ X kj (c * a), X jk b]) as W2. rewrite CL6 -?ST0' Zdef' in HeqW2.
-remember ([ ~ X ik (a * b), X ki c]) as W3. rewrite CL6 -?ST0' Zdef in HeqW3.
+move: A0. rewrite /HW ?ST1 ?conj_com -?ST0' ?GII ?invI ?ST1 ?cmul_r 
+ ST1' (ST1' ik) (ST1' ji) ?comm_conj -?ST0' ?ST2' ?conj_com -?ST0' ?invI ?ST1 ?mul_inv ?inv_mul -?mul_assoc
+ ?cmul_l // (ST1 ki) (ST1 ij) (ST1 jk) /conj -?ST0' ?invI.
+remember ([ ~ X ji (b * c), X ij a]) as W1. rewrite comm_d1 -?ST0' Zdef in HeqW1.
+remember ([ ~ X kj (c * a), X jk b]) as W2. rewrite comm_d2 -?ST0' Zdef' in HeqW2.
+remember ([ ~ X ik (a * b), X ki c]) as W3. rewrite comm_d2 -?ST0' Zdef in HeqW3.
 rewrite ?ST0'. cancellate. rewrite -?GA -?ST0' HeqW1 HeqW2 HeqW3.
 remember (Z ij _ _) as Z1. remember (Z ik _ _) as Z2. remember (Z (swap_neq jk) _ _) as Z3.
 by rewrite -?GA /RHS ?HeqZ1 ?HeqZ2 ?HeqZ3. Qed.
