Group.v
@@ -1,0 +1,98 @@
+Require Import ssreflect ssrnat ssrbool seq eqtype.
+
+Module Type GroupCarrier.
+
+Parameter ZZ : Type.
+
+End GroupCarrier.
+
+Module GroupFacts (carrier : GroupCarrier).
+Import carrier.
+
+(* Group Structure *)
+Variable (group_mul : ZZ -> ZZ -> ZZ) (groupinv : ZZ -> ZZ) (Id : ZZ).
+
+Notation "x .* y " := (group_mul x y) (at level 50, left associativity).
+Notation "x ^-1" := (groupinv x) (at level 40).
+
+(* Group axioms *)
+Axiom GA : forall g1 g2 g3, g1 .* g2 .* g3 = g1 .* (g2 .* g3).
+Axiom GId: forall g, g .* Id = g.
+Axiom IdG: forall g, Id .* g = g.
+Axiom GI : forall g, g .* (g ^-1) = Id.
+Axiom IG: forall g, (g ^-1) .* g = Id.
+
+(* Basic lemmata *)
+
+Corollary GI' g A: g .* ((g ^-1) .* A) = A. by rewrite -GA GI IdG. Qed.
+
+Corollary IG' g A: (g^-1) .* (g .* A) = A. by rewrite -GA IG IdG. Qed.
+
+Lemma GC: forall g3 g1 g2, g1 .* g3 = g2 .* g3 -> g1 = g2.
+intros. have: (g1 .* g3 .* g3 ^-1 = g2 .* g3 .* g3 ^-1) by rewrite H.
+by rewrite ?GA ?GI ?GId. Qed.
+
+Lemma GIM: forall g1 g2, (g1 .* g2) ^-1 = g2 ^-1 .* g1 ^-1.
+intros. apply (GC (g1 .* g2)). by rewrite IG GA -(GA (g1 ^-1)) IG IdG IG. Qed.
+
+Lemma GII: forall g, g ^-1 ^-1 = g.
+intros. apply (GC (g^-1)). by rewrite IG GI. Qed.
+
+Lemma IdI: Id ^-1 = Id. apply (GC Id). by rewrite IG IdG. Qed.
+
+(* Conjugate elements *)
+
+Definition conj (h g : ZZ) := (g ^-1) .* h .* g.
+Notation "h ^ g" := (conj h g).
+
+Lemma conj_mul h g1 g2: h ^ (g1 .* g2) = (h ^ g1) ^ g2.
+by rewrite /conj ?GIM ?GA. Qed.
+
+Lemma mul_conj g h1 h2: (h1 .* h2) ^ g = h1 ^ g .* h2 ^ g.
+by rewrite /conj ?GA -(GA g) GI IdG. Qed.
+
+Lemma conjId g: g ^ Id = g.
+by rewrite /conj IdI IdG GId. Qed.
+
+(* Commutators *)
+
+Definition Comm (x y : ZZ) : ZZ := (x .* y .* x^-1 .* y^-1).
+Notation "[ ~ x1 , x2 , .. , xn ]" :=
+  (Comm .. (Comm x1 x2) .. xn) (at level 29, left associativity).
+
+Lemma Comm_inv: forall x y, [~ x, y] ^-1 = [~y, x].
+intros. by rewrite /Comm ?GIM ?GII -?GA. Qed.
+
+Lemma conj_com: forall a b, a ^ b = [~ b ^-1, a] .* a. 
+intros. rewrite /conj. apply (GC Id). by rewrite -{1}(IG a) -GA /Comm GII GId. Qed. 
+
+Ltac expand := rewrite /Comm /conj ?GIM ?GII.
+Ltac cancel := rewrite ?GI' ?IG' ?GI ?IG.
+Ltac cancellate := expand; rewrite ?GA; cancel.
+
+Lemma comm3 x y z: [~z, x, y]^ z = [~x, z^-1, y^z]. by cancellate. Qed.
+
+Lemma cmul_l x y z: [~ x .* y, z] = [~y, z] ^ (x^-1) .* [~x, z]. by cancellate. Qed.
+
+Lemma cmul_r x y z: [~ x, y .* z] = [~x, y] .* [~x, z] ^ (y^-1). by cancellate. Qed.
+
+Lemma comm_conj x y z: [~ x, y] ^ z = [~x ^ z, y ^ z]. by cancellate. Qed.
+
+Lemma comm_d1 x y: [~ x, y] = y ^ (x^-1) .* y^-1. by expand. Qed.
+
+Lemma comm_d2 x y: [~ x, y] = x .* (x^-1) ^ (y^-1). by cancellate. Qed.
+
+(* Variations of Hall-Witt identity*)
+
+Lemma HallWitt x y z: 
+ [~ y^-1, x, z] ^ (y^-1) .* [~ z^-1, y, x] ^ (z^-1) .* [~ x^-1, z, y] ^ (x^-1) = Id. 
+ by expand; rewrite ?GA; do 4 cancel. Qed.
+
+Corollary HallWitt' x y z: [~ y, x^-1, z^-1]^ y .* [~z, y^-1, x^-1]^ z .* [~x, z^-1, y^-1] ^ x = Id.
+move: (HallWitt (x^-1) (y^-1) (z^-1)). by rewrite ?GII. Qed.
+
+Corollary HallWitt'' x y z:
+ [~ x^-1, y^-1, (z^-1)^y] .* [~ y^-1, z^-1, (x^-1)^z] .* [~ z^-1, x^-1, (y^-1)^x] = Id. 
+by rewrite -?comm3 HallWitt'. Qed.
+
+End GroupFacts.
